feat[ident]: fresh_seq of nfresh

theories/common/ident.v
@@ -311,7 +311,7 @@ Coercion bLatticeType : type >-> Order.BLattice.type.
 Coercion distrLatticeType : type >-> Order.DistrLattice.type.
 Coercion bDistrLatticeType : type >-> Order.BDistrLattice.type.
 Coercion wfType : type >-> WellFounded.type.
-(* Coercion orderType : type >-> Order.TOrder.type. *)
+Coercion orderType : type >-> Order.Total.type.
 
 End Exports.
 
@@ -454,10 +454,10 @@ Proof.
   move=>->; rewrite encode_fresh -(inj_eq encode_inj); lia.
 Qed.
 
-Import Order.
+Import Order.Exports.
 
 Definition fresh_seq : seq T -> T := fun t => 
-  fresh (foldr Order.max \i0 t).
+  fresh (max_seq (\i0 : T) t).
 
 Lemma fresh_seq_nil : 
   fresh_seq [::] = (\i1 : T).
@@ -484,7 +484,6 @@ Proof.
   rewrite ?maxEle -fresh_mon; by case: ifP.
 Qed.
 
-
 Lemma fresh_seq_mem x s : 
   x \in s -> x <^i fresh_seq s.
 Proof. 
@@ -500,17 +499,19 @@ Qed.
 Lemma fresh_seq_nmem s : fresh_seq s \notin s.
 Proof. by apply/memPn => x /fresh_seq_mem; rewrite lt_neqAle=> /andP[]. Qed.
 
-(* Lemma fresh_seq_nfresh x n : 
-  0 < n -> fresh_seq (nfresh x n) = iter n fresh x.
-Proof. 
-  rewrite /fresh_seq foldl_maxn_sorted; last first.
-  - rewrite sorted_map; apply /sub_sorted /nfresh_sorted.
-    rewrite /ident_lt /= /Def.ident_lt=> {}x y /=; exact /ltW.
-  have {2}->: 0%nat = @encode T \i0 by apply/esym/encode0.
-  rewrite last_map; case: n=> [|{}n].
-  - by rewrite encode0=> /=. 
-  by rewrite nfreshSr last_rcons iterS /fresh.
-Qed. *)
+Section fresh_seq_nfresh.
+
+Arguments nfresh : simpl never.
+
+Lemma fresh_seq_nfresh x n : 
+  n != 0 -> fresh_seq (nfresh x n) = iter n fresh x.
+Proof.
+  case: n=> //= n _; rewrite /fresh_seq; apply/congr1/eqP/max_seqP=> //.
+  split=>>; first by apply/path.trajectP; exists n.
+  rewrite in_nfresh /(_ <=^i _) /= /Def.ident_le encode_iter; lia.
+Qed.
+
+End fresh_seq_nfresh.
 
 Lemma mem_le_max s x: 
   x \in s -> x <= foldr ident_max \i0 s.
